src/typechecker/FStarC.TypeChecker.TcEffect.fsti
@@ -24,14 +24,14 @@ module S = FStarC.Syntax.Syntax
 module Env = FStarC.TypeChecker.Env
 
 
-val dmff_cps_and_elaborate : Env.env -> S.eff_decl -> (list S.sigelt & S.eff_decl & option S.sigelt)
+val dmff_cps_and_elaborate : Env.env -> S.eff_decl -> ML (list S.sigelt & S.eff_decl & option S.sigelt)
 
-val tc_eff_decl : Env.env -> S.eff_decl -> list S.qualifier -> list S.attribute -> S.eff_decl
+val tc_eff_decl : Env.env -> S.eff_decl -> list S.qualifier -> list S.attribute -> ML S.eff_decl
 
-val tc_lift : Env.env -> S.sub_eff -> Range.t -> S.sub_eff
+val tc_lift : Env.env -> S.sub_eff -> Range.t -> ML S.sub_eff
 
-val tc_effect_abbrev : Env.env -> (lident & S.univ_names & S.binders & S.comp) -> Range.t -> (lident & S.univ_names & S.binders & S.comp)
+val tc_effect_abbrev : Env.env -> (lident & S.univ_names & S.binders & S.comp) -> Range.t -> ML (lident & S.univ_names & S.binders & S.comp)
 
-val tc_polymonadic_bind : Env.env -> m:lident -> n:lident -> p:lident -> bind_t:S.tscheme -> S.tscheme & S.tscheme & S.indexed_effect_combinator_kind
+val tc_polymonadic_bind : Env.env -> m:lident -> n:lident -> p:lident -> bind_t:S.tscheme -> ML (S.tscheme & S.tscheme & S.indexed_effect_combinator_kind)
 
-val tc_polymonadic_subcomp : Env.env -> m:lident -> n:lident -> subcomp_t:S.tscheme -> S.tscheme & S.tscheme & S.indexed_effect_combinator_kind
+val tc_polymonadic_subcomp : Env.env -> m:lident -> n:lident -> subcomp_t:S.tscheme -> ML (S.tscheme & S.tscheme & S.indexed_effect_combinator_kind)
